tla/MC_SATBFinalRemarkPremarked.tla
@@ -1,0 +1,3 @@
+----------------------- MODULE MC_SATBFinalRemarkPremarked -----------------------
+EXTENDS SATBFinalRemarkPremarked
+=============================================================================
